Finperm/Function/Fin.lean
@@ -1,0 +1,70 @@
+/-
+Copyright (c) 2026 Kry10. All rights reserved.
+Released under Apache 2.0 license as described in the file LICENSE.
+Authors: Wrenna Robson
+-/
+module
+
+public import Batteries.Data.Fin.Lemmas
+import Finperm.Function.Swap
+
+@[expose] public section
+
+namespace Function
+
+theorem RightInverse.leftInverse_of_surjective {f : α → β} {g : β → α} :
+    RightInverse f g → Surjective f → LeftInverse f g :=
+  fun h hg x ↦ let ⟨y, hy⟩ := hg x; hy ▸ congrArg f (h y)
+
+def finInv (f : Fin n → Fin n) : Fin n → Fin n := fun i => (Fin.find? (f · == i)).getD i
+
+theorem apply_finInv_eq_of_apply_eq {f : Fin n → Fin n} (hf : f j = i) :
+    f (finInv f i) = i := by
+  have h : (Fin.find? (f · == i)).isSome := Fin.isSome_find?_of_eq_true (beq_of_eq hf)
+  rw [finInv, ← beq_iff_eq, ← Option.get_eq_getD (Fin.find? (f · == i)) (h := h),
+    Fin.get_find?_eq_true h]
+
+theorem Surjective.rightInverse_finInv {f : Fin n → Fin n} (hf : f.Surjective) :
+    (finInv f).RightInverse f := fun i => apply_finInv_eq_of_apply_eq (hf i).choose_spec
+
+theorem Injective.leftInverse_finInv {f : Fin n → Fin n} (hf : f.Injective) :
+    (finInv f).LeftInverse f := fun _ => hf (apply_finInv_eq_of_apply_eq rfl)
+
+theorem Surjective.injective_finInv {f : Fin n → Fin n} (hf : f.Surjective) :
+    (finInv f).Injective := hf.rightInverse_finInv.injective
+
+theorem Injective.surjective_finInv {f : Fin n → Fin n} (hf : f.Injective) :
+    (finInv f).Surjective := RightInverse.surjective hf.leftInverse_finInv
+
+open Fin in
+theorem Injective.surjectiveOfFin {f : Fin n → Fin n} (hf : f.Injective) : f.Surjective := by
+  induction n with
+  | zero => exact (·.elim0)
+  | succ n IH =>
+    let g := swapVal (last n) (f (last n))
+    have hgf : Surjective (g ∘ f) := by
+      apply Fin.lastCases
+      · exact ⟨last n, swapVal_apply_right _ _⟩
+      · intro i
+        let F (j : Fin n) : Fin n := ((g ∘ f) j.castSucc).castLT (val_lt_last <| by grind)
+        have hF : F.Injective := by grind [Function.Injective]
+        exact (IH hF i).imp' Fin.castSucc (fun _ => Fin.ext ∘ congrArg (@Fin.val n))
+    exact fun a => (hgf (g a)).imp fun _ hx => swapVal_injective hx
+
+theorem Injective.rightInverse_finInv {f : Fin n → Fin n} (hf : f.Injective) :
+    (finInv f).RightInverse f := hf.surjectiveOfFin.rightInverse_finInv
+
+theorem Surjective.surjective_finInv {f : Fin n → Fin n} (hf : f.Surjective) :
+    (finInv f).Surjective := hf.injective_finInv.surjectiveOfFin
+
+theorem Surjective.leftInverse_finInv {f : Fin n → Fin n} (hf : f.Surjective) :
+    (finInv f).LeftInverse f :=
+  hf.rightInverse_finInv.leftInverse_of_surjective hf.surjective_finInv
+
+theorem Surjective.injectiveOfFin {f : Fin n → Fin n} (hf : f.Surjective) : f.Injective :=
+  hf.leftInverse_finInv.injective
+
+theorem Injective.injective_finInv {f : Fin n → Fin n} (hf : f.Injective) :
+    (finInv f).Injective := hf.surjective_finInv.injectiveOfFin
+
+end Function
