Finperm/Vector/Nodup.lean
@@ -1,0 +1,40 @@
+/-
+Copyright (c) 2026 Kry10. All rights reserved.
+Released under Apache 2.0 license as described in the file LICENSE.
+Authors: Wrenna Robson
+-/
+namespace Vector
+
+def Nodup (v : Vector α n) : Prop := v.toList.Nodup
+
+theorem nodup_iff_toList_nodup {v : Vector α n} : v.Nodup ↔ v.toList.Nodup := Iff.rfl
+
+theorem nodup_iff_eq_of_getElem_eq {v : Vector α n} : v.Nodup ↔
+    ∀ (i j : Nat) (_hi : i < n) (_hj : j < n), v[i] = v[j] → i = j :=
+  v.nodup_iff_toList_nodup.trans <| List.nodup_iff_eq_of_getElem_eq.trans <| by simp
+
+theorem Nodup.eq_of_getElem_eq {v : Vector α n} (h : Nodup v) (hi : i < n)
+    (hj : j < n) : v[i] = v[j] → i = j := nodup_iff_eq_of_getElem_eq.mp h _ _ _ _
+
+theorem Nodup.eq_of_getElem?_eq {v : Vector α n} (h : Nodup v) (hi : i < n)
+    (hij : v[i]? = v[j]?) : i = j := by
+  simp [getElem?_def, hi] at hij
+  rcases hij with ⟨hj, hij⟩
+  exact h.eq_of_getElem_eq hi hj hij
+
+@[simp, grind =] theorem Nodup.getElem_inj {v : Vector α n} (h : Nodup v) {hi : i < n}
+    {hj : j < n} : v[i] = v[j] ↔ i = j := ⟨h.eq_of_getElem_eq hi hj, (getElem_congr rfl · hi)⟩
+
+theorem Nodup.getElem?_inj {v : Vector α n} (h₀ : i < n) (h₁ : v.Nodup) :
+    v[i]? = v[j]? ↔ i = j := by
+  simp [h₀, getElem?_eq_some_iff, h₁.getElem_inj, eq_comm]
+  exact fun h => h ▸ h₀
+
+theorem Nodup.getD_inj {v : Vector α n}
+    (h₀ : i < n) (h₁ : j < n) (h₂ : Nodup v) :
+    v.getD i fallback = v.getD j fallback ↔ i = j := by
+  simp [getD, h₀, h₁, h₂.getElem_inj]
+
+theorem Nodup.getElem!_inj [Inhabited α] {v : Vector α n}
+    (h₀ : i < n) (h₁ : j < n) (h₂ : Nodup v) : v[i]! = v[j]! ↔ i = j := by
+  simp [h₀, h₁, h₂.getElem_inj]
